Listed all lemmas we should try to prove about the primitive generators

src/SemGen.v
@@ -1,5 +1,5 @@
 Require Import ZArith List ssreflect ssrbool ssrnat.
-Require Import Axioms RoseTrees Random AbstractGen Gen.
+Require Import Axioms RoseTrees Random Gen.
 Import ListNotations.
 
 Set Implicit Arguments.
@@ -11,7 +11,7 @@ Definition unGen {A : Type} (g : Gen A) : RandomGen -> nat -> A :=
   match g with MkGen f => f end.
 
 Definition semGen {A : Type} (g : Gen A) : Ensemble A :=
-  fun a => exists seed, exists size, (unGen g) seed size = a.
+  fun a => exists size, exists seed, (unGen g) seed size = a.
 
 (* Equivalence on sets of outcomes *)
 Definition set_eq {A} (m1 m2 : Ensemble A) :=
@@ -19,17 +19,23 @@ Definition set_eq {A} (m1 m2 : Ensemble A) :=
 
 Infix "<-->" := set_eq (at level 70, no associativity) : pred_scope.
 
+(* the set f outcomes m1 is a subset of m2 *)
+Definition set_incl {A} (m1 m2 : Ensemble A) :=
+  forall A, m1 A -> m2 A.
+
+Infix "-->" := set_incl (at level 70, no associativity) : pred_scope.
+
 Open Scope pred_scope.
 
 Axiom randomSeedInhabitant : RandomGen.
 
-Lemma semReturn : forall {A} (x : A),
+Lemma semReturn : forall A (x : A),
   semGen (returnG x) <--> eq x.
 Proof.
   move => A x a. rewrite /semGen. split.
-  - move => [seed [size H]] //.
+  - move => [size [seed H]] //.
   - move => H /=. rewrite H.
-    exists randomSeedInhabitant. exists 0. reflexivity.
+    exists 0. exists randomSeedInhabitant. reflexivity.
 Qed.
 
 (* This seems like a very strong assumption;
@@ -40,29 +46,77 @@ Axiom rndSplitAssumption :
 (* We will clearly need to reason about sizes:
    generators need to be size-monotonous functions *)
 (* Currently can't assume this of all generators,
-   but this will probably need to be part of Gen (sigma type?)
-   / or of some type class(Arbitrary?) *)
-Axiom genSize : forall {A : Type} (a : A) g seed1 size1 size2,
+   but this will probably need to be part of Gen
+   (sigma type? this would break the non-intrusiveness of our solution)
+   / or of some type class (Arbitrary? a super class if it so that
+   users can choose how much they want to prove) *)
+Axiom genSize : forall A (a : A) g seed1 size1 size2,
   (size1 <= size2)%coq_nat ->
   (unGen g) seed1 size1 = a ->
   exists seed2, (unGen g) seed2 size2 = a.
 
-Lemma semBind : forall {A B} (g : Gen A) (f : A -> Gen B),
+Lemma semBind : forall A B (g : Gen A) (f : A -> Gen B),
   semGen (bindG g f) <--> fun b => exists a, (semGen g) a /\ (semGen (f a)) b.
 Proof.
   move => A B g f b. rewrite /semGen /bindG => /=. split.
-  - case : g => [g] /= [seed [size H]]. move : H.
+  - case : g => [g] /= [size [seed H]]. move : H.
     case (rndSplit seed) => [seed1 seed2].
     exists (g seed1 size). split; do 2 eexists. reflexivity.
     rewrite <- H. case (f (g seed1 size)). reflexivity.
-  - move => [a [[seed1 [size1 H1]] [seed2 [size2 H2]]]].
+  - move => [a [[size1 [seed1 H1]] [size2 [seed2 H2]]]].
     assert (Hs1 : (size1 <= max size1 size2)%coq_nat) by apply Max.le_max_l.
     case (genSize _ _ Hs1 H1) => [seed1' H1'].
     assert (Hs2 : (size2 <= max size1 size2)%coq_nat) by apply Max.le_max_r.
     case (genSize _ _ Hs2 H2) => [seed2' H2'].
-    clear H1 H2.
+    eexists (max size1 size2). clear H1 H2.
     case (rndSplitAssumption seed1' seed2') => [seed Hs].
-    exists seed. eexists (max size1 size2).
+    exists seed.
     move : H1' H2'. case : g => [g] /= H1' H2'.
     rewrite Hs. rewrite H1'. move : H2'. by case (f a).
 Qed.
+
+Lemma semFMap : forall A B (f : A -> B) (g : Gen A),
+  semGen (fmapG f g) = semGen (bindG g (fun a => returnG (f a))).
+Proof.
+  (* Should be able to prove this without any extra axioms!? *)
+Admitted.
+
+Lemma semChoose : forall A `{Random A} a1 a2,
+  semGen (chooseG (a1,a2)) <--> (fun a => Random.leq a1 a /\ Random.leq a a2).
+Proof.
+  move => A H a1 a2. rewrite /semGen. simpl.
+  admit. (* this seems like a reasonable thing to assume of randomR,
+            why not add it directly to the Random type class? *)
+Admitted.
+
+Lemma semSized : forall A (f : nat -> Gen A),
+  (forall size1 size2,
+    (size1 <= size2)%coq_nat -> semGen (f size2) --> semGen (f size2)) ->
+  semGen (sizedG f) <--> (fun a => exists n, semGen (f n) a).
+Proof.
+  move => A f Mon a. rewrite /semGen /sizedG => /=. split.
+  - move => [size [seed H]]. exists size. move : H.
+    case (f size) => g H. by eauto.
+  - move => [n [size [seed H]]].
+    exists (max n size).
+    admit. (* Hopefully this follows from something like Mon *)
+Admitted.
+
+Lemma semSuchThatMaybe : forall A (g : Gen A) (f : A -> bool),
+  semGen (suchThatMaybeG g f) <-->
+  (fun o => (o = None) \/ (exists y, o = Some y /\ semGen g y /\ f y)).
+Proof.
+  move => A g f a. rewrite /suchThatMaybeG.
+  admit. (* looks a bit scarry *)
+Admitted.
+
+Lemma semPromote : forall A (m : Rose (Gen A)),
+  semGen (promoteG m) <-->
+  match m with
+    | MkRose g _ =>
+      semGen(bindG g (fun x : A => returnG (MkRose x (lazy nil))))
+  end.
+Proof.
+  move => A m a. rewrite /promoteG /fmapRose.
+  admit. (* looks a bit scarry *)
+Admitted.
